search for blocking flows in residual gaph reduced to simple graph (backward translation still missing), acyclicity of level graph proven, more distance lemmas.

Dinic/Compute_Blocking_Residual.thy
@@ -1,33 +1,50 @@
 theory Compute_Blocking_Residual
   imports DFS_Collect_Backtrack_Example Compute_Blocking_Simple "HOL-Library.Product_Lexorder"
+    Graph_Algorithms_Dev.BFS_Example
 begin
+  (*TODO MOVE*)
+lemma vwalk_bet_diff_verts_length_geq_2:"vwalk_bet E s  p t\<Longrightarrow> s \<noteq> t \<Longrightarrow> length p \<ge> 2"
+  by(cases p rule: edges_of_vwalk.cases) (auto simp add: vwalk_bet_def)
 
+lemma same_graph_consts: "G.graph_inv = dfs.Graph.graph_inv"
+  "G.digraph_abs = dfs.Graph.digraph_abs"
+  "BFS_Example.neighbourhood = dfs.Graph.neighbourhood"
+  "DFS_Collect_Backtrack_Example.neighbourhood = 
+                          dfs.Graph.neighbourhood"
+  "G.graph_inv = dfs.Graph.graph_inv"
+      apply (auto simp add: adj_inv_def RBT_Set.empty_def
+      BFS_Example.neighbourhood_def DFS_Collect_Backtrack_Example.neighbourhood_def
+      )
+
+
+
+  done
 global_interpretation blocking_simple: blocking_simple where insert = vset_insert and
- sel = sel and  vset_empty = vset_empty and  diff = vset_diff and
- lookup = lookup and empty = map_empty and delete=delete and isin = isin and t_set=t_set
-and update=update and adjmap_inv = adj_inv and vset_delete= vset_delete
-and vset_inv = vset_inv and union=vset_union and inter=vset_inter 
-and flow_lookup = lookup
-and flow_empty = Leaf
-and flow_update=update
-and flow_delete=delete
-and flow_invar=adj_inv
-and G = G and
-t = t and
-s = s and
-find_path = find_path and
-u = u
+  sel = sel and  vset_empty = vset_empty and  diff = vset_diff and
+  lookup = lookup and empty = map_empty and delete=delete and isin = isin and t_set=t_set
+  and update=update and adjmap_inv = adj_inv and vset_delete= vset_delete
+  and vset_inv = vset_inv and union=vset_union and inter=vset_inter 
+  and flow_lookup = lookup
+  and flow_empty = Leaf
+  and flow_update=update
+  and flow_delete=delete
+  and flow_invar=adj_inv
+  and G = G and
+  t = t and
+  s = s and
+  find_path = find_path and
+  u = u
 for G s t find_path u
 defines blocking_simple_loop=blocking_simple.compute_blocking_loop_impl
-and     blocking_simple_initial=blocking_simple.initial_state
-and add_flow_simple=blocking_simple.add_flow
-and delete_edge=blocking_simple.delete_edge
+  and     blocking_simple_initial=blocking_simple.initial_state
+  and add_flow_simple=blocking_simple.add_flow
+  and delete_edge=blocking_simple.delete_edge
   by(auto intro!: blocking_simple.intro
-           simp add: dfs.Graph.Pair_Graph_Specs_axioms  dfs.set_ops.Set2_axioms
-                      M.Map_axioms[simplified RBT_Set.empty_def adj_inv_def[symmetric]])
+      simp add: dfs.Graph.Pair_Graph_Specs_axioms  dfs.set_ops.Set2_axioms
+      M.Map_axioms[simplified RBT_Set.empty_def adj_inv_def[symmetric]])
 
 definition "find_path F s t = 
-   (if neighbourhood F s = vset_empty then None
+   (if DFS_Collect_Backtrack_Example.neighbourhood F s = vset_empty then None
     else let final_state = dfs_del_dead_impl F t ( dfs_backtrack_initial_state s)
          in  (case return final_state of NotReachable \<Rightarrow> None |
                                          Reachable    \<Rightarrow> 
@@ -44,23 +61,23 @@ value "inorder (flow (blocking_simple_loop 0 10 find_path (\<lambda> e. 4) (bloc
 hide_const G edges
 
 lemma find_path_correct:
-assumes "dfs.Graph.graph_inv F" "dfs.Graph.finite_graph F" "dfs.Graph.finite_vsets F" "s \<noteq> t"
-shows "\<exists>p. vwalk_bet (dfs.Graph.digraph_abs F) s p t \<Longrightarrow>
+  assumes "dfs.Graph.graph_inv F" "dfs.Graph.finite_graph F" "dfs.Graph.finite_vsets F" "s \<noteq> t"
+  shows "\<exists>p. vwalk_bet (dfs.Graph.digraph_abs F) s p t \<Longrightarrow>
        \<exists>p del. vwalk_bet (dfs.Graph.digraph_abs F) s p t \<and> find_path F s t = Some (p, del)"
-       (is "?asm1 \<Longrightarrow> ?thesis1")
-      "find_path F s t = Some (p, dlt) \<Longrightarrow>
+    (is "?asm1 \<Longrightarrow> ?thesis1")
+    "find_path F s t = Some (p, dlt) \<Longrightarrow>
        acyc (dfs.Graph.digraph_abs F) \<Longrightarrow>
        vwalk_bet (dfs.Graph.digraph_abs F) s p t \<and>
        distinct p \<and>
        (\<forall>e\<in>set dlt. \<nexists>p. e \<in> set (edges_of_vwalk p) \<and> vwalk_bet (dfs.Graph.digraph_abs F) s p t)"
-       (is "?asm2 \<Longrightarrow> ?asm3 \<Longrightarrow> ?thesis2")
-proof(all \<open>cases "neighbourhood F s = vset_empty"\<close>)
- show  "?asm1 \<Longrightarrow> ?thesis1" if asy: "neighbourhood F s = vset_empty"
-   using assms(4) dfs.Graph.vset.set.set_empty vwalk_then_edge[of "dfs.Graph.digraph_abs F" s _  t] 
-   by(unfold dfs.Graph.are_connected_abs[OF assms(1), symmetric] asy) blast
-  show  "?asm2 \<Longrightarrow> ?asm3 \<Longrightarrow> ?thesis2"  if asy: "neighbourhood F s = vset_empty"
+    (is "?asm2 \<Longrightarrow> ?asm3 \<Longrightarrow> ?thesis2")
+proof(all \<open>cases "DFS_Collect_Backtrack_Example.neighbourhood F s = vset_empty"\<close>)
+  show  "?asm1 \<Longrightarrow> ?thesis1" if asy: "DFS_Collect_Backtrack_Example.neighbourhood F s = vset_empty"
+    using assms(4) dfs.Graph.vset.set.set_empty vwalk_then_edge[of "dfs.Graph.digraph_abs F" s _  t] 
+    by(unfold dfs.Graph.are_connected_abs[OF assms(1), symmetric] asy) blast
+  show  "?asm2 \<Longrightarrow> ?asm3 \<Longrightarrow> ?thesis2"  if asy: "DFS_Collect_Backtrack_Example.neighbourhood F s = vset_empty"
     using asy by(simp add: find_path_def)
-  assume s_neighb_non_empty:"neighbourhood F s \<noteq> vset_empty"
+  assume s_neighb_non_empty:"DFS_Collect_Backtrack_Example.neighbourhood F s \<noteq> vset_empty"
   have DFS_axioms: "DFS.DFS_axioms isin t_set adj_inv vset_empty vset_inv lookup F s"
     using RBT_Set.empty_def Tree2.eq_set_tree_empty assms(1,2,3)  s_neighb_non_empty
     by(auto intro:dfs.Graph.neighbourhood_absD simp add: dfs.DFS_axioms_def)
@@ -70,7 +87,7 @@ proof(all \<open>cases "neighbourhood F s = vset_empty"\<close>)
   have same_final_state: "dfs_del_dead_impl F t ( dfs_backtrack_initial_state s) =
                          dfs.DFS_collect_backtrack F t ( dfs_backtrack_initial_state s)"
     by(simp add: dfs_del_dead_impl_def dfs_backtrack_initial_state_def
-                 DFS_thms.DFS_collect_backtrack_impl_same_on_initial[OF dfs_thms]) 
+        DFS_thms.DFS_collect_backtrack_impl_same_on_initial[OF dfs_thms]) 
   have same_final_as_ordinary: "to_ordinary_DFS_state 
                     (dfs.DFS_collect_backtrack F t ( dfs_backtrack_initial_state s)) =
                     dfs.DFS F t ( dfs.initial_state s)"
@@ -89,7 +106,7 @@ proof(all \<open>cases "neighbourhood F s = vset_empty"\<close>)
       by(auto simp add: final_state_def)
     show ?case 
     proof(rule exI[of _ "rev (stack final_state)"], rule exI[of _ "backtrack final_state"],
-            rule conjI, goal_cases)
+        rule conjI, goal_cases)
       case 2
       then show ?case
         using s_neighb_non_empty dfs_backtrack_reachable 
@@ -104,31 +121,260 @@ proof(all \<open>cases "neighbourhood F s = vset_empty"\<close>)
   show  "?asm2 \<Longrightarrow> ?asm3 \<Longrightarrow> ?thesis2"
   proof(goal_cases)
     case 1
-     define final_state where "final_state = dfs_del_dead_impl F t ( dfs_backtrack_initial_state s)"
-     have dfs_backtrack_result: "return final_state =  Reachable" "rev (stack final_state) = p" 
-                                "backtrack final_state = dlt"
-     apply(all \<open>rule case_split[of "DFS_Collect_Backtrack_Example.neighbourhood F s = vset_empty"]\<close>)
-     apply(all \<open>rule return.exhaust[of "DFS_backtrack_state.return (dfs_del_dead_impl
+    define final_state where "final_state = dfs_del_dead_impl F t ( dfs_backtrack_initial_state s)"
+    have dfs_backtrack_result: "return final_state =  Reachable" "rev (stack final_state) = p" 
+      "backtrack final_state = dlt"
+        apply(all \<open>rule case_split[of "DFS_Collect_Backtrack_Example.neighbourhood F s = vset_empty"]\<close>)
+           apply(all \<open>rule return.exhaust[of "DFS_backtrack_state.return (dfs_del_dead_impl
                          F t (dfs_backtrack_initial_state s))"]\<close>)
-     using "1"(1) 
-     by(auto simp add: final_state_def find_path_def) 
-   have "vwalk_bet (dfs.Graph.digraph_abs F) s p t"
-     using DFS_correct_2[of t]  dfs_backtrack_result(1) dfs_backtrack_result(2)       
-     by(auto simp add: final_state_def same_final_state same_final_as_ordinary[symmetric])
-   moreover have "distinct p" 
-     using DFS_thms.invar_seen_stack_holds[OF dfs_thms 
-                                    DFS_thms.initial_state_props(6,1,3)[OF dfs_thms], of t]
-     by(simp add: dfs.invar_seen_stack_def same_final_as_ordinary[symmetric]
-                   dfs_backtrack_result(2)[symmetric] final_state_def same_final_state)
-   moreover have "e\<in>set dlt \<Longrightarrow>
+      using "1"(1) 
+      by(auto simp add: final_state_def find_path_def) 
+    have "vwalk_bet (dfs.Graph.digraph_abs F) s p t"
+      using DFS_correct_2[of t]  dfs_backtrack_result(1) dfs_backtrack_result(2)       
+      by(auto simp add: final_state_def same_final_state same_final_as_ordinary[symmetric])
+    moreover have "distinct p" 
+      using DFS_thms.invar_seen_stack_holds[OF dfs_thms 
+          DFS_thms.initial_state_props(6,1,3)[OF dfs_thms], of t]
+      by(simp add: dfs.invar_seen_stack_def same_final_as_ordinary[symmetric]
+          dfs_backtrack_result(2)[symmetric] final_state_def same_final_state)
+    moreover have "e\<in>set dlt \<Longrightarrow>
                   \<nexists>p. e \<in> set (edges_of_vwalk p) \<and> vwalk_bet (dfs.Graph.digraph_abs F) s p t" for e
-     using  same_final_state  "1"(2) DFS_thms.dfs_backtrack_final(5)[OF dfs_thms, of t]       
-     by(simp add: dfs.invar_dfs_backtrack_5_def acyc_def  dfs_backtrack_initial_state_def 
-                  final_state_def  dfs_backtrack_result(2,3)[symmetric])     
-   ultimately show ?case by auto
- qed
+      using  same_final_state  "1"(2) DFS_thms.dfs_backtrack_final(5)[OF dfs_thms, of t]       
+      by(simp add: dfs.invar_dfs_backtrack_5_def acyc_def  dfs_backtrack_initial_state_def 
+          final_state_def  dfs_backtrack_result(2,3)[symmetric])     
+    ultimately show ?case by auto
+  qed
 qed
 
+
+locale blocking_level_residual_spec =
+  flow_network_spec where fst = fst  +
+  Map_realising: Map realising_edges_empty 
+  "realising_edges_update::('v\<times> 'v) \<Rightarrow> ('e Redge) list \<Rightarrow> 'realising_type \<Rightarrow> 'realising_type"
+  realising_edges_delete realising_edges_lookup realising_edges_invar +
+  Map_residual_flow: Map residual_flow_empty
+  "residual_flow_update::'e Redge \<Rightarrow> real \<Rightarrow> 'resflow_map \<Rightarrow> 'resflow_map"
+  residual_flow_delete residual_flow_lookup residual_flow_invar
+
+for fst::"'e \<Rightarrow> 'v::linorder" and realising_edges_empty realising_edges_update
+  realising_edges_delete realising_edges_lookup realising_edges_invar
+  residual_flow_delete residual_flow_lookup residual_flow_invar residual_flow_empty
+  residual_flow_update  +
+fixes s t ::'v
+  and   es::"'e list"
+  and   \<f>::"'e \<Rightarrow> real"
+begin
+
+definition "pos_es = filter (\<lambda> e. rcap \<f> e > 0) (map F es @ map B es)"
+
+definition "realising_edges_general list =
+           (foldr (\<lambda> e found_edges. let ee = to_vertex_pair e in
+                     (case realising_edges_lookup found_edges ee of 
+                      None \<Rightarrow> realising_edges_update ee [e] found_edges
+                     |Some ds \<Rightarrow> realising_edges_update ee (e#ds) found_edges))
+            list realising_edges_empty)"
+
+definition "realising_edges = realising_edges_general pos_es"
+
+definition "E_simple = foldr (\<lambda> e acc. add_edge acc (prod.fst e) (prod.snd e))
+                          (map to_vertex_pair pos_es) empty"
+
+definition "level_simple = parents (bfs_impl E_simple (bfs_initial_state 
+                          (vset_insert s Pair_Graph_RBT.vset_empty)))"
+
+definition "u_simple e = sum_list (map (\<lambda> e. real_of_ereal (rcap \<f> e)) 
+                       (case realising_edges_lookup realising_edges e of None \<Rightarrow> []| 
+                        Some ees \<Rightarrow> ees))"
+
+definition "blocking_flow_simple = 
+      (if neighbourhood E_simple s = vset_empty 
+       then None
+       else let f = flow (blocking_simple_loop s t find_path u_simple 
+                 (blocking_simple_initial level_simple))
+            in if f = empty then None
+            else Some f)"
+
+definition "residual_add_flow f e \<gamma> = 
+residual_flow_update e ((abstract_real_map (residual_flow_lookup f) e) + \<gamma>) f"
+
+definition "residual_blocking_flow =
+    (case blocking_flow_simple 
+     of None \<Rightarrow> None |
+        Some flw \<Rightarrow>
+     Some (
+       foldr 
+          (\<lambda> e acc. 
+             prod.fst 
+              (
+               foldr 
+                 (\<lambda> ee (resf, f). 
+                  let \<gamma> = min (real_of_ereal (rcap \<f> ee)) (abstract_real_map (lookup f) e)
+                  in (residual_add_flow resf ee \<gamma>, add_flow_simple f (-\<gamma>) e))
+                 (the (realising_edges_lookup realising_edges e)) 
+                 (acc, flw)
+              )
+          )
+         (map to_vertex_pair pos_es)
+         residual_flow_empty
+      ))"
+
+
+end
+
+locale blocking_level_residual= 
+  blocking_level_residual_spec +
+  flow_network+
+  assumes es_props: "set es = \<E>" "distinct es"
+  assumes s_neq_t: "s \<noteq> t"
+  assumes finite_capacities: "\<And> e. e \<in> \<E> \<Longrightarrow> \<u> e < \<infinity>"
+begin
+
+lemma finite_rescaps: "e \<in> \<EE> \<Longrightarrow> rcap f e < \<infinity>"  "e \<in> \<EE> \<Longrightarrow> rcap f e > - \<infinity>"
+  using finite_capacities 
+  by(auto simp add:  \<EE>_def minus_ereal_def u_non_neg)
+
+lemma finite_rescapsE: "e \<in> \<EE> \<Longrightarrow>(\<And> r. rcap f e  = ereal r \<Longrightarrow> P) \<Longrightarrow> P"
+  using finite_rescaps[of e f] 
+  by(cases "rcap f e" rule: real_of_ereal.cases) auto
+
+lemma pos_es_props: "set pos_es = {e | e. e \<in> \<EE> \<and> rcap \<f> e > 0}"
+  "distinct pos_es"
+  by (auto intro!: distinct_filter inj_onI 
+      simp add: pos_es_def \<EE>_def  distinct_map es_props)
+
+lemma realising_edges_invar_pres: "realising_edges_invar (realising_edges_general list)"
+  unfolding realising_edges_general_def
+  by(auto intro: foldr_invar 
+      simp add: Map_realising.invar_empty Map_realising.invar_update realising_edges_general_def 
+      split: option.split)
+
+lemma realising_edges_general_result_None_and_Some:
+  assumes "(case realising_edges_lookup (realising_edges_general list) (u, v) 
+            of Some ds \<Rightarrow> ds 
+               | None \<Rightarrow> [])= ds"
+  shows "set ds = {e | e. e \<in> set list \<and> to_vertex_pair e = (u, v)}"
+  using assms
+proof(induction list arbitrary: ds)
+  case Nil
+  then show ?case 
+    by (auto simp add: realising_edges_general_def  Map_realising.map_empty 
+        split: option.split)
+next
+  case (Cons a list ds)
+  show ?case 
+    using Map_realising.map_update[OF  realising_edges_invar_pres] Cons(1)[OF refl] 
+    by (auto intro: realising_edges_invar_pres 
+        simp add: Map_realising.map_update realising_edges_general_def Cons(2)[symmetric] 
+        split: option.split)
+qed
+
+lemma realising_edges_general_result_distinct:
+  assumes "distinct list"
+    "(case realising_edges_lookup (realising_edges_general list) (u, v) 
+            of Some ds \<Rightarrow> ds 
+               | None \<Rightarrow> [])= ds"
+  shows "distinct ds"
+  using assms
+proof(induction list arbitrary: ds u v)
+  case Nil
+  then show ?case 
+    by (auto simp add: realising_edges_general_def  Map_realising.map_empty 
+        split: option.split)
+next
+  case (Cons e list ds u v)
+  hence distlist: "distinct list" by auto
+  show ?case 
+    using  realising_edges_general_result_None_and_Some[OF Cons(3)]  Cons(1)[OF distlist refl, of u v]
+    unfolding realising_edges_general_def Cons(3)[symmetric]
+    apply(subst (asm) foldr_Cons, subst (asm) o_apply)
+    apply(subst (asm) foldr_Cons, subst (asm) o_apply)
+    apply(subst foldr_Cons, subst  o_apply)
+    unfolding realising_edges_general_def[symmetric]
+    using Cons(1)[OF distlist refl, of u v]  Cons.prems(1) 
+      realising_edges_general_result_None_and_Some[OF refl, of list u v]
+    by (auto simp add: realising_edges_general_def[symmetric] 
+        Map_realising.map_update[OF  realising_edges_invar_pres , of "to_vertex_pair e" _ list] 
+        split: option.split)
+qed
+
+lemma realising_edges_general_result:
+  assumes "realising_edges_lookup (realising_edges_general list) (u, v) = Some ds"
+  shows "set ds = {e | e. e \<in> set list \<and> to_vertex_pair e = (u, v)}"
+  using realising_edges_general_result_None_and_Some[of list u v ds] assms
+  by simp
+
+lemma realising_edges_result:
+  "realising_edges_lookup realising_edges (u, v) = Some ds \<Longrightarrow>
+    set ds = {e |e. e \<in> set pos_es \<and> to_vertex_pair e = (u, v)}"
+  "realising_edges_lookup realising_edges (u, v) = Some ds \<Longrightarrow>
+    distinct ds"
+  "realising_edges_lookup realising_edges (u, v) = None \<Longrightarrow>
+    {e |e. e \<in> set pos_es \<and> to_vertex_pair e = (u, v)} = {}"
+  using realising_edges_general_result_distinct[OF pos_es_props(2) refl, of u v] 
+    realising_edges_general_result_None_and_Some[OF refl] 
+  by(force simp add: realising_edges_def realising_edges_general_result)+
+
+lemma E_simple_props: "dfs.Graph.graph_inv E_simple" (is ?goal1)
+  "dfs.Graph.finite_graph E_simple" (is ?goal2)
+  "dfs.Graph.finite_vsets E_simple" (is ?goal3)
+  "dfs.Graph.digraph_abs E_simple = to_vertex_pair ` (set pos_es)" (is ?goal4)
+proof-
+  define init where "init = (vset_empty:: (('b \<times> ('b \<times> color) tree) \<times> color) tree)"
+  define list where "list = pos_es"
+  have init_props: "dfs.Graph.graph_inv init" "dfs.Graph.finite_graph init" 
+    "dfs.Graph.finite_vsets init"
+    "dfs.Graph.digraph_abs init = to_vertex_pair ` (set [])"
+    by (auto simp add: G.graph_inv_empty adj_inv_def init_def
+        M.map_empty dfs.Graph.finite_graphI  empty_digraph_abs)
+
+  have "?goal1 \<and> ?goal2 \<and> ?goal3 \<and> ?goal4"
+    unfolding E_simple_def init_def[symmetric] list_def[symmetric]
+    using init_props 
+    by(induction list)(auto intro: dfs.Graph.finite_graph_add_edge)
+  thus ?goal1 ?goal2 ?goal3 ?goal4 by auto
+qed
+
+lemma u_simple_is:
+  "u_simple (u, v) = (\<Sum>e\<in>{e |e. e \<in> set pos_es \<and> to_vertex_pair e = (u, v)}.
+                          real_of_ereal \<uu>\<^bsub>\<f>\<^esub>e)"
+  using realising_edges_result[of u v]
+  by(auto intro!: comm_monoid_add_class.sum.neutral 
+      split: option.split 
+      simp add: u_simple_def,
+      simp only: comm_monoid_add_class.sum.distinct_set_conv_list[symmetric])
+
+lemma u_strictly_pos:
+  "e \<in> dfs.Graph.digraph_abs E_simple \<Longrightarrow> u_simple e > 0"
+  using finite_rescaps(1) zero_less_real_of_ereal 
+  by  (cases e)
+    (auto intro!: ordered_comm_monoid_add_class.sum_pos 
+      intro: finite_rescapsE 
+      simp add: u_simple_is pos_es_props(1) E_simple_props(4) finite_\<EE>)
+
+lemma u_non_neg:
+  "u_simple e \<ge> 0"
+  by(cases e)
+    (auto intro!: ordered_comm_monoid_add_class.sum_nonneg
+      simp add: u_simple_is pos_es_props(1) E_simple_props(4) finite_\<EE> real_of_ereal_pos)
+
+lemma bfs_axiom: "neighbourhood E_simple s \<noteq>vset_empty \<Longrightarrow>
+                 BFS.BFS_axiom isin t_set M.invar \<langle>\<rangle> vset_inv lookup
+                   (vset_insert s Pair_Graph_RBT.vset_empty) E_simple"
+  unfolding BFS.BFS_axiom_def[OF bfs.BFS_axioms]
+  using E_simple_props(1-3) 
+  by (auto simp add: dfs.Graph.vset.set.set_insert[OF  dfs.Graph.vset.set.invar_empty]
+      dfs.Graph.vset.set.set_empty dfs.Graph.vset.set.invar_empty
+      Tree2.finite_set_tree[of "DFS_Collect_Backtrack_Example.neighbourhood 
+                                                  E_simple _", 
+        simplified dfs.Graph.neighbourhood_abs[OF  E_simple_props(1)]]
+      same_graph_consts(1-3))
+    (*
+lemma level_siple_is: "(bfs_impl E_simple (bfs_initial_state 
+                          (vset_insert s Pair_Graph_RBT.vset_empty))) = 
+                       (bfs.BFS E_simple (bfs_initial_state 
+                          (vset_insert s Pair_Graph_RBT.vset_empty)))"
+*)
+    (*
 interpretation blocking_simple_thms: blocking_simple_thms where insert = vset_insert and
  sel = sel and  vset_empty = vset_empty and  diff = vset_diff and
  lookup = lookup and empty = map_empty and delete=delete and isin = isin and t_set=t_set
@@ -139,13 +385,230 @@ and flow_empty = Leaf
 and flow_update=update
 and flow_delete=delete
 and flow_invar=adj_inv
-and G = G and
+and G = E_simple and
 t = t and
 s = s and
 find_path = find_path and
 u = u
-for G s t u
   apply(auto intro!: blocking_simple_thms.intro) 
   apply (simp add: blocking_simple.flow_map.Map_axioms blocking_simple.intro
       dfs.Graph.Pair_Graph_Specs_axioms dfs.set_ops.Set2_axioms)
-  apply(rule blocking_simple_thms_axioms.intro)
+  apply(auto intro!: blocking_simple_thms_axioms.intro simp add: E_simple_props)
+  apply (simp add: E_simple_props(1))*)
+
+lemma e_leaving_s_in_level_graph:
+  "e\<in>\<EE> \<Longrightarrow> 0 < \<uu>\<^bsub>\<f>\<^esub>e \<Longrightarrow> fstv e = s \<Longrightarrow> sndv e \<noteq> s \<Longrightarrow>
+   to_vertex_pair e \<in> level_graph (to_vertex_pair ` {e |e. e \<in> \<EE> \<and> 0 < \<uu>\<^bsub>\<f>\<^esub>e}) {s} -
+    {(u, v) |u v. distance (to_vertex_pair ` {e |e. e \<in> \<EE> \<and> 0 < \<uu>\<^bsub>\<f>\<^esub>e}) s u = \<infinity>}"
+  apply(cases "to_vertex_pair e")
+  by(subst distance_0I[OF refl, of "fstv e"] |
+      auto intro!: in_level_graphI exI[of _e]  exI[of _ "0::nat"] 
+      intro: distance_1I 
+      simp add: enat_0  image_iff distance_set_single_source to_vertex_pair_fst_snd)+
+
+lemma has_elem_not_emptyI:"x \<in> A \<Longrightarrow> A \<noteq> {}"
+  by auto
+
+lemma flow_network_axioms_for_simple_graph:
+  "(\<exists> e\<in> \<EE>. rcap \<f> e > 0 \<and> fstv e = s \<and> sndv e \<noteq> s) \<Longrightarrow>
+         flow_network prod.fst prod.snd id Pair (\<lambda>x. ereal (u_simple x))
+     (level_graph (dfs.Graph.digraph_abs E_simple) {s} -
+      {(u, v) |u v. distance (dfs.Graph.digraph_abs E_simple) s u = \<infinity>})"
+  apply(rule flow_network.intro)
+   apply(rule  multigraph.intro)
+      apply (force simp add: id_def, force simp add: id_def)
+    apply(rule finite_Diff)
+    apply(rule finite_subset[OF level_graph_subset_graph])
+    apply(simp add: E_simple_props(4))
+  using has_elem_not_emptyI[OF  e_leaving_s_in_level_graph]
+  by(auto intro: flow_network_axioms.intro has_elem_not_emptyI
+      simp add: u_non_neg  E_simple_props(4) pos_es_props(1))
+
+abbreviation "simple_level_graph_abstract ==  (level_graph (dfs.Graph.digraph_abs E_simple) {s}
+     - {(u, v) | u v. distance  (dfs.Graph.digraph_abs E_simple) s u = \<infinity>})"
+abbreviation "is_blocking_flow_simple == flow_network.is_blocking_flow prod.fst prod.snd id u_simple 
+     simple_level_graph_abstract"
+
+lemma "blocking_flow_simple = None \<Longrightarrow> \<nexists> p. vwalk_bet (dfs.Graph.digraph_abs E_simple) s p t" (is "?none \<Longrightarrow> ?nowalk")
+  "blocking_flow_simple = Some f \<Longrightarrow>\<exists> p. vwalk_bet (dfs.Graph.digraph_abs E_simple) s p t" (is "?some \<Longrightarrow> ?walk")
+  "blocking_flow_simple = Some f \<Longrightarrow> is_blocking_flow_simple s t (abstract_real_map (lookup f))" (is "?some \<Longrightarrow> ?blocking_flow")
+  "blocking_flow_simple = Some f \<Longrightarrow>\<exists>e\<in>\<EE>. 0 < \<uu>\<^bsub>\<f>\<^esub>e \<and> fstv e = s \<and> sndv e \<noteq> s" (is "?some \<Longrightarrow>?leaving_e")
+proof(all \<open>cases "neighbourhood E_simple s = vset_empty"\<close>)
+  show "?none \<Longrightarrow> neighbourhood E_simple s = vset_empty \<Longrightarrow> ?nowalk"
+    by (auto simp add: G.source_of_path_neighb_non_empty RBT_Set.empty_def s_neq_t
+        vwalk_bet_diff_verts_length_geq_2  dfs.Graph.neighbourhood_def
+        DFS_Collect_Backtrack_Example.neighbourhood_def
+        blocking_flow_simple_def same_graph_consts(3))
+  show "?some \<Longrightarrow> neighbourhood E_simple s = vset_empty \<Longrightarrow> ?walk"
+    by (auto simp add:  blocking_flow_simple_def )   
+  show "?some \<Longrightarrow> neighbourhood E_simple s = vset_empty \<Longrightarrow> ?blocking_flow"
+    by (auto simp add:  blocking_flow_simple_def )
+  show "?some \<Longrightarrow> BFS_Example.neighbourhood E_simple s = vset_empty \<Longrightarrow> \<exists>e\<in>\<EE>. 0 < \<uu>\<^bsub>\<f>\<^esub>e \<and> fstv e = s \<and> sndv e \<noteq> s"
+    by (auto simp add:  blocking_flow_simple_def )  
+  assume assm1: "neighbourhood E_simple s \<noteq> vset_empty"
+  note bfs_axiom = bfs_axiom[OF assm1]
+  have level_siple_is: "(bfs_impl E_simple (bfs_initial_state 
+                          (vset_insert s Pair_Graph_RBT.vset_empty))) = 
+                       (bfs.BFS E_simple (bfs_initial_state 
+                          (vset_insert s Pair_Graph_RBT.vset_empty)))"
+    by (simp add: bfs.BFS_impl_same bfs_axiom)
+  have sources: "t_set (vset_insert s vset_empty) = {s}"
+    "s \<in> t_set (vset_insert s vset_empty)"
+    by (auto simp add: dfs.Graph.vset.set.invar_empty dfs.Graph.vset.set.set_empty)
+  note BFS_correct_1 = bfs.BFS_correct_1[OF bfs_axiom sources(2)]
+  note BFS_correct_2 = bfs.BFS_correct_2[OF bfs_axiom]
+  note BFS_correct_3 = bfs.BFS_correct_3[OF bfs_axiom sources(2)]
+  note BFS_correct_4 = bfs.BFS_correct_4[OF bfs_axiom]
+  note BFS_level_graph = bfs.BFS_level_graph[OF bfs_axiom]
+  note bfs_initial_state_props = bfs.initial_state_props[OF bfs_axiom]
+  have bfs_invar_1: "bfs.invar_1 (bfs.BFS E_simple (bfs_initial_state 
+                          (vset_insert s Pair_Graph_RBT.vset_empty)))"
+    using bfs.invar_1_holds[OF bfs_axiom] bfs_initial_state_props(1,4) by blast
+  have bfs_invar_2: "bfs.invar_2 (vset_insert s Pair_Graph_RBT.vset_empty) 
+                          E_simple (bfs.BFS E_simple (bfs_initial_state 
+                          (vset_insert s Pair_Graph_RBT.vset_empty)))"
+    by (simp add: bfs.invar_2_holds bfs_axiom bfs_initial_state_props(1))
+
+  define prnts where "prnts =  parents ((bfs.BFS E_simple (bfs_initial_state 
+                          (vset_insert s Pair_Graph_RBT.vset_empty))))"
+  have acyc_bfs_result:
+    "acyc (dfs.Graph.digraph_abs prnts)"
+    using reachable_level_graph_acyclic
+    by(force simp add: prnts_def bfs.BFS_level_graph[OF bfs_axiom, simplified same_graph_consts] acyc_def reachable_level_graph_def)
+
+  have blocking_simple_thms: "blocking_simple_thms map_empty RBT_Map.delete vset_insert isin t_set sel 
+                   update adj_inv vset_empty vset_delete vset_inv vset_union vset_inter vset_diff
+                   lookup lookup \<langle>\<rangle> update RBT_Map.delete adj_inv prnts s t u_simple find_path"
+  proof(rule  blocking_simple_thms.intro[OF blocking_simple.blocking_simple_axioms],
+      rule blocking_simple_thms_axioms.intro, goal_cases)
+    case 1
+    then show ?case 
+      using bfs_invar_1[simplified bfs.invar_1_def]
+      by (simp add: adj_inv_def prnts_def)
+  next
+    case 2
+    then show ?case 
+      using bfs_invar_1[simplified bfs.invar_1_def]
+      by (simp add: adj_inv_def prnts_def)
+  next
+    case 3
+    then show ?case 
+      using Tree2.finite_set_tree by blast
+  next
+    case 4
+    then show ?case 
+      using acyc_bfs_result by auto
+  next
+    case (5 e)
+    then show ?case 
+      using BFS_correct_4 
+      by(cases e)(auto intro!: u_strictly_pos simp add: RBT_Set.empty_def prnts_def subset_iff)
+  next
+    case (6 e)
+    then show ?case
+      by (simp add: u_non_neg)
+  next
+    case 7
+    then show ?case 
+      by (simp add: s_neq_t)
+  next
+    case (8 F s t)
+    then show ?case
+      using find_path_correct(1) by blast
+  next
+    case (9 F s t p del)
+    then show ?case 
+      using find_path_correct(2) by blast
+  qed
+
+  note blocking_simple_correctness=blocking_simple_thms.correctness[OF blocking_simple_thms]
+
+  show none_no_walk:"?none \<Longrightarrow> ?nowalk"
+  proof(goal_cases)
+    case 1
+    hence flow_empty:"blocking_state.flow 
+           (blocking_simple_loop s t find_path u_simple 
+                 (blocking_simple_initial level_simple)) = empty"
+      using assm1
+      by (auto simp add:  blocking_flow_simple_def )
+    have no_parent_path:"\<nexists>p. vwalk_bet (dfs.Graph.digraph_abs prnts) s p t"
+      using flow_empty  blocking_simple_correctness(4) level_siple_is 
+      by(intro blocking_simple_correctness(1)) 
+        (auto simp add: blocking_simple.termination_same RBT_Set.empty_def blocking_simple_initial_def 
+          level_simple_def  prnts_def)    
+    show ?case 
+    proof(rule ccontr, goal_cases)
+      case 1
+      have "\<exists>q . vwalk_bet (G.digraph_abs prnts) s q t"
+        using  bfs.BFS_graph_path_implies_parent_path[OF bfs_axiom] 1 s_neq_t sources(1,2)
+        by(force simp add: RBT_Set.empty_def  prnts_def)
+      thus ?case
+        using no_parent_path
+        by (simp add: RBT_Set.empty_def)
+    qed
+  qed
+  assume assms2: "blocking_flow_simple = Some f" "BFS_Example.neighbourhood E_simple s \<noteq> vset_empty"
+  have asm2': "BFS_Example.neighbourhood E_simple s \<noteq> \<langle>\<rangle>" 
+    "BFS_Example.neighbourhood E_simple s \<noteq> vset_empty"
+    using assm1 by auto
+  have parent_path:"\<exists>p. vwalk_bet (dfs.Graph.digraph_abs prnts) s p t"   
+    using assms2(1)  level_siple_is not_None_eq[of blocking_flow_simple] 
+      Compute_Blocking_Residual.blocking_simple.termination_same[OF blocking_simple_correctness(4), symmetric]     
+    by(intro blocking_simple_correctness(2)) 
+      (auto simp add: if_not_P[OF asm2'(1)] prnts_def blocking_flow_simple_def
+        blocking_simple_initial_def level_simple_def RBT_Set.empty_def) 
+  show has_path:"\<exists>p. vwalk_bet (dfs.Graph.digraph_abs E_simple) s p t"
+    using BFS_correct_4  parent_path 
+    by(auto intro!:  vwalk_bet_subset simp add: RBT_Set.empty_def prnts_def)
+  then obtain p where p_prop: "vwalk_bet (dfs.Graph.digraph_abs E_simple) s p t" "distinct p"
+    using  vwalk_bet_to_distinct_is_distinct_vwalk_bet by(force simp add: distinct_vwalk_bet_def)
+
+  have srcs_are_s:"t_set (vset_insert s vset_empty) = {s}"
+    using sources(1) by blast
+
+  show residual_leaving_s:"\<exists>e\<in>\<EE>. 0 < \<uu>\<^bsub>\<f>\<^esub>e \<and> fstv e = s \<and> sndv e \<noteq> s" 
+  proof-
+    obtain x where x_prop:"hd (edges_of_vwalk p) = (s, x)" "(s, x) \<in> dfs.Graph.digraph_abs E_simple "
+      using  s_neq_t by(auto intro: vwalk_betE[OF p_prop(1)])
+    then obtain e where e_prop:"0 < \<uu>\<^bsub>\<f>\<^esub>e" "(s, x) = to_vertex_pair e" "e\<in>\<EE>"
+      by(auto simp add: E_simple_props(4) pos_es_props(1))
+    moreover hence "fstv e = s"  
+      using  fst_eqD[of s x] vs_to_vertex_pair_pres(1) by simp
+    moreover have "sndv e \<noteq> s" 
+    proof(rule ccontr, goal_cases)
+      case 1
+      hence "\<exists> xs. p = [s,s]@xs"
+        using p_prop(1,2) fst_eqD[of s x] vs_to_vertex_pair_pres(1) e_prop(2) x_prop(1) s_neq_t
+        by(cases p rule: edges_of_vwalk.cases, all \<open>cases e\<close>)
+          (auto simp add: vwalk_bet_def vs_to_vertex_pair_pres split_pairs)
+      thus False
+        using p_prop(2) by force
+    qed
+    ultimately show ?thesis by auto
+  qed
+  note  flow_network_axioms_for_simple_graph = 
+    flow_network_axioms_for_simple_graph[OF residual_leaving_s]
+  note is_blocking_flow_def=flow_network.is_blocking_flow_def[OF  flow_network_axioms_for_simple_graph]
+  note bfs_level_graph_def=BFS_level_graph[simplified same_graph_consts(2) srcs_are_s 
+      distance_set_single_source, symmetric]
+  have flow_non_empt: "blocking_state.flow (blocking_simple_loop s t find_path u_simple 
+                 (blocking_simple_initial level_simple)) \<noteq> Leaf"
+    using  assms2(1)
+    by(auto simp add: blocking_flow_simple_def if_not_P[OF assm1] RBT_Set.empty_def[symmetric]) 
+  note same_final_state =
+    Compute_Blocking_Residual.blocking_simple.termination_same[OF blocking_simple_correctness(4)]
+  note flow_non_empt'=flow_non_empt[simplified blocking_simple_loop_def parents_def[symmetric]]
+  note same_final_state'= same_final_state[simplified parents_def[symmetric] blocking_simple_loop_def]
+
+  show "is_blocking_flow_simple s t (abstract_real_map (lookup f))"
+    using same_final_state blocking_simple_correctness(3) assms2(1)
+      flow_non_empt is_blocking_flow_def[of s t]  not_None_eq option.inject
+    by(unfold prnts_def level_siple_is level_simple_def  blocking_simple_initial_def
+        blocking_flow_simple_def  bfs_level_graph_def if_not_P[OF assm1] Let_def,
+        subst (asm) if_not_P)
+      (auto simp add: if_not_P)
+qed
+
+
+end
+end
