Mincost_Flow_Algorithms/Use_Orlins_Algorithm/Instantiation.thy
@@ -925,7 +925,7 @@ abbreviation "\<cc> \<equiv> cost_flow_network.\<cc>"
 abbreviation "F \<equiv> flow_network_spec.F"
 abbreviation "B \<equiv> flow_network_spec.B"
 abbreviation "to_edge == cost_flow_network.to_vertex_pair"
-abbreviation "oedge == cost_flow_network.oedge"
+abbreviation "oedge == flow_network_spec.oedge"
 abbreviation "rcap == cost_flow_network.rcap"
 
 lemma default_conv_to_rdg: "cost_flow_network.consist default_conv_to_rdg"
@@ -1485,7 +1485,7 @@ proof(goal_cases)
           ({cost_flow_network.F d |d. d \<in> local.\<E>} \<union> {cost_flow_network.B d |d. d \<in> local.\<E>})"
     for a b x
   by (smt (verit, del_insts) cost_flow_network.\<EE>_def cost_flow_network.o_edge_res
-    cost_flow_network.oedge_simps'(2) cost_flow_network.to_vertex_pair.simps(2) image_iff swap_simp)
+    flow_network_spec.oedge_simps'(2) cost_flow_network.to_vertex_pair.simps(2) image_iff swap_simp)
     show ?case
     by(auto simp add: cost_flow_network.to_vertex_pair.simps es_is_E EEE_def cost_flow_network.\<EE>_def
           intro: help1 help2 help3) 
@@ -2081,8 +2081,8 @@ next
     using 2  bellman_ford.weight.simps[OF bellman_ford]  
     by(auto simp add: arc_implies_awalk get_edge_and_costs_forward_result_props)
     moreover have "(\<forall>e\<in>set (map (\<lambda>e. prod.fst (get_edge_and_costs_forward nb f (prod.fst e) (prod.snd e))) ppp).
-        nb (flow_network.oedge e) \<and> 0 < cost_flow_network.rcap f e)"
-      using 2  bellman_ford.weight.simps[OF bellman_ford] cost_flow_network.oedge_simps'
+        nb (flow_network_spec.oedge e) \<and> 0 < cost_flow_network.rcap f e)"
+      using 2  bellman_ford.weight.simps[OF bellman_ford] flow_network_spec.oedge_simps'
                 cost_flow_network.rcap.simps get_edge_and_costs_forward_result_props[OF sym[OF prod.collapse], of nb f x y]
       by(auto simp add: \<u>_def)
     ultimately show ?case by simp
@@ -2106,9 +2106,9 @@ ereal
     using  "3.prems"(1) bellman_ford.weight.simps[OF bellman_ford]
     by (simp add: get_edge_and_costs_forward_result_props)
   moreover have "(\<forall>e\<in>set (map (\<lambda>e. prod.fst (get_edge_and_costs_forward nb f (prod.fst e) (prod.snd e))) (edges_of_vwalk (y # xs))).
-    nb (flow_network.oedge e) \<and> 0 < cost_flow_network.rcap f e)" 
+    nb (flow_network_spec.oedge e) \<and> 0 < cost_flow_network.rcap f e)" 
     by (simp add: "3.IH" calculation(3))
-  moreover have "nb (flow_network.oedge (prod.fst (get_edge_and_costs_forward nb f x y)))"
+  moreover have "nb (flow_network_spec.oedge (prod.fst (get_edge_and_costs_forward nb f x y)))"
     using  "3.prems"(1) bellman_ford.weight.simps[OF bellman_ford]
              get_edge_and_costs_forward_result_props[OF prod.collapse[symmetric], of nb f x y]
     by auto
@@ -2143,7 +2143,7 @@ proof(rule nexistsI, goal_cases)
       "(\<And> e. e\<in>set (map (\<lambda>e. prod.fst (get_edge_and_costs_forward (not_blocked state) (current_flow state) (prod.fst e)
                          (prod.snd e)))
            (edges_of_vwalk c)) \<Longrightarrow>
-        not_blocked state (flow_network.oedge e) \<and> 0 < cost_flow_network.rcap (current_flow state) e)"
+        not_blocked state (flow_network_spec.oedge e) \<and> 0 < cost_flow_network.rcap (current_flow state) e)"
     using path_bf_flow_network_path[OF _ length_c weight_le_PInfty refl] by auto
   define cc where "cc = (map (\<lambda>e. prod.fst (get_edge_and_costs_forward (not_blocked state) (current_flow state) (prod.fst e) (prod.snd e)))
                        (edges_of_vwalk c))"
@@ -2242,7 +2242,7 @@ proof(rule if_E[where P= "\<lambda> x. t = x"], fast, goal_cases)
   from 1 have knowledge: "get_source state \<in> VV"
     "aux_invar state"
     "(\<forall>e\<in>to_rdgs to_pair (conv_to_rdg state) (Adj_Map_Specs2.to_graph  (\<FF>_imp state)).
-        0 < current_flow state (flow_network.oedge e))"
+        0 < current_flow state (flow_network_spec.oedge e))"
     "invar_isOptflow state" 
     "(\<exists>t\<in>VV. balance state t < - (\<epsilon> * current_\<gamma> state) \<and> resreach (current_flow state) s t)"
     by force+
@@ -2261,13 +2261,13 @@ proof(rule if_E[where P= "\<lambda> x. t = x"], fast, goal_cases)
   ultimately obtain pp where pp_prop:"augpath (current_flow state) pp"
      "fstv (hd pp) = s" "sndv (last pp) = tt"
      "set pp
-     \<subseteq> {e |e. e \<in> EEE \<and> cost_flow_network.oedge e \<in> to_set (actives state)} \<union> to_rdgs to_pair (conv_to_rdg state) (\<FF> state)"
+     \<subseteq> {e |e. e \<in> EEE \<and> flow_network_spec.oedge e \<in> to_set (actives state)} \<union> to_rdgs to_pair (conv_to_rdg state) (\<FF> state)"
      "foldr (\<lambda>x. (+) (\<cc> x)) pp 0 \<le> foldr (\<lambda>x. (+) (\<cc> x)) p 0"
     using  algo.simulate_inactives_costs[ of "current_flow state" p, of s tt state, OF _ _ _ _ _  refl refl refl refl refl refl refl refl ]
            1(8) by auto
   have F_is: "\<FF> state = to_graph (\<FF>_imp state)" 
     using knowledge(2) from_aux_invar'(21) by auto
-  hence e_in:"e \<in> set pp \<Longrightarrow> e \<in> {e |e. e \<in> EEE \<and> cost_flow_network.oedge e \<in> to_set (actives state)} 
+  hence e_in:"e \<in> set pp \<Longrightarrow> e \<in> {e |e. e \<in> EEE \<and> flow_network_spec.oedge e \<in> to_set (actives state)} 
                    \<union> to_rdgs to_pair (conv_to_rdg state) (\<FF> state)" for e
       using pp_prop(4)  by auto
     hence e_es:"e \<in> set pp \<Longrightarrow> cost_flow_network.to_vertex_pair e \<in> set es" for e
@@ -2284,7 +2284,7 @@ proof(rule if_E[where P= "\<lambda> x. t = x"], fast, goal_cases)
       using oedge_where from_aux_invar'(1,3)[OF knowledge(2)] by auto
     have posflow:"\<exists> d. e = B d \<Longrightarrow> current_flow state (oedge e) > 0" 
       using cost_flow_network.augpath_rcap_pos_strict'[OF  pp_prop(1) 1]
-      by(induction  rule: cost_flow_network.oedge.cases[OF  , of e])
+      by(induction  rule: flow_network_spec.oedge.cases[OF  , of e])
          auto
     have "prod.snd (get_edge_and_costs_forward (not_blocked state) (current_flow state)
      (fstv e) (sndv e)) \<le> \<cc> e"
@@ -2363,7 +2363,7 @@ proof(rule if_E[where P= "\<lambda> x. t = x"], fast, goal_cases)
          (\<forall>e\<in>set (map (\<lambda>e. prod.fst (get_edge_and_costs_forward (not_blocked state) (current_flow state) (prod.fst e)
                          (prod.snd e)))
            (edges_of_vwalk Pbf)).
-    not_blocked state (flow_network.oedge e) \<and> 0 < cost_flow_network.rcap (current_flow state) e)"
+    not_blocked state (flow_network_spec.oedge e) \<and> 0 < cost_flow_network.rcap (current_flow state) e)"
     by(intro path_bf_flow_network_path[OF _ length_Pbf weight_le_PInfty refl]) simp
   hence Pbf_props: "awalk UNIV (hd Pbf) (edges_of_vwalk Pbf) (last Pbf)"
                    " weight (not_blocked state) (current_flow state) Pbf =
@@ -2373,7 +2373,7 @@ proof(rule if_E[where P= "\<lambda> x. t = x"], fast, goal_cases)
                    "(\<And> e. e \<in> set (map (\<lambda>e. prod.fst (get_edge_and_costs_forward (not_blocked state) (current_flow state) (prod.fst e)
                          (prod.snd e)))
            (edges_of_vwalk Pbf)) \<Longrightarrow>
-    not_blocked state (flow_network.oedge e) \<and> 0 < cost_flow_network.rcap (current_flow state) e)"
+    not_blocked state (flow_network_spec.oedge e) \<and> 0 < cost_flow_network.rcap (current_flow state) e)"
     by auto
   define P where "P = (map (\<lambda>e. prod.fst (get_edge_and_costs_forward (not_blocked state) (current_flow state) (prod.fst e) (prod.snd e)))
                    (edges_of_vwalk Pbf))"
@@ -2467,7 +2467,7 @@ qed
 
 lemma bf_weight_leq_res_costs:
 assumes "set (map oedge qq) \<subseteq> set \<E>_list"
-        " \<And> e. e \<in> set qq \<Longrightarrow> not_blocked state (flow_network.oedge e)"
+        " \<And> e. e \<in> set qq \<Longrightarrow> not_blocked state (flow_network_spec.oedge e)"
         "\<And> e. e \<in> set qq \<Longrightarrow> 0 < cost_flow_network.rcap (current_flow state) e"
         "unconstrained_awalk (map cost_flow_network.to_vertex_pair qq)"
    and  qq_len: "length qq \<ge> 1"
@@ -2580,7 +2580,7 @@ lemma get_source_target_path_a_ax:
   assumes "get_source_target_path_a_cond  state s t P b \<gamma> f"
   shows "0 < cost_flow_network.Rcap f (set P) \<and>
         (invar_isOptflow state \<longrightarrow> cost_flow_network.is_min_path f s t P) \<and>
-         cost_flow_network.oedge ` set P \<subseteq> to_set (actives state) \<union> \<F> state \<and>
+         flow_network_spec.oedge ` set P \<subseteq> to_set (actives state) \<union> \<F> state \<and>
          distinct P"
   apply(insert assms)
   unfolding  loopB.get_source_target_path_a_cond_def
@@ -2614,7 +2614,7 @@ proof(cases "invar_isOptflow state", goal_cases)
        insert "1"(1), unfold get_target_for_source_def, presburger+)
   hence 
     "(\<forall>e\<in>to_rdgs to_pair (conv_to_rdg state) (to_graph (\<FF>_imp state)).
-        0 < current_flow state (flow_network.oedge e))"
+        0 < current_flow state (flow_network_spec.oedge e))"
     by auto
   have  loopB_call1_cond: " loopB_call1_cond state"
     using  1 unfolding loopB.loopB_call1_cond_def by presburger
@@ -2643,7 +2643,7 @@ proof(cases "invar_isOptflow state", goal_cases)
      "fstv (hd qq) = s"
      "sndv (last qq) = t"
      "set qq
-     \<subseteq> {e |e. e \<in> EEE \<and> cost_flow_network.oedge e \<in> to_set (actives state)} \<union>
+     \<subseteq> {e |e. e \<in> EEE \<and> flow_network_spec.oedge e \<in> to_set (actives state)} \<union>
         to_rdgs to_pair (conv_to_rdg state) (\<FF> state)"
      "foldr (\<lambda>x. (+) (\<cc> x)) qq 0 \<le> foldr (\<lambda>x. (+) (\<cc> x)) Q 0" "qq \<noteq> []"
   using algo.simulate_inactives_costs[OF  Q_prop(1-4) knowledge(5)
@@ -2654,7 +2654,7 @@ proof(cases "invar_isOptflow state", goal_cases)
     by(cases qq rule: list_cases3) auto
   have F_is: "\<FF> state = to_graph (\<FF>_imp state)" 
     by (simp add: "1"(1) from_aux_invar'(21))
-  hence e_in:"e \<in> set qq \<Longrightarrow> e \<in> {e |e. e \<in> EEE \<and> cost_flow_network.oedge e \<in> to_set (actives state)} 
+  hence e_in:"e \<in> set qq \<Longrightarrow> e \<in> {e |e. e \<in> EEE \<and> flow_network_spec.oedge e \<in> to_set (actives state)} 
                    \<union> to_rdgs to_pair (conv_to_rdg state) (\<FF> state)" for e
       using qq_prop(4)  by auto
     hence e_es:"e \<in> set qq \<Longrightarrow> cost_flow_network.to_vertex_pair e \<in> set es" for e
@@ -2757,7 +2757,7 @@ proof(cases "invar_isOptflow state", goal_cases)
          (\<forall>e\<in>set (map (\<lambda>e. prod.fst (get_edge_and_costs_forward (not_blocked state) (current_flow state) (prod.fst e)
                          (prod.snd e)))
            (edges_of_vwalk Pbf)).
-    not_blocked state (flow_network.oedge e) \<and> 0 < cost_flow_network.rcap (current_flow state) e)"
+    not_blocked state (flow_network_spec.oedge e) \<and> 0 < cost_flow_network.rcap (current_flow state) e)"
     by(intro path_bf_flow_network_path[OF _ length_Pbf weight_le_PInfty refl]) simp
   hence Pbf_props: "awalk UNIV (hd Pbf) (edges_of_vwalk Pbf) (last Pbf)"
                    " weight (not_blocked state) (current_flow state) Pbf =
@@ -2767,7 +2767,7 @@ proof(cases "invar_isOptflow state", goal_cases)
                    "(\<And> e. e \<in> set (map (\<lambda>e. prod.fst (get_edge_and_costs_forward (not_blocked state) (current_flow state) (prod.fst e)
                          (prod.snd e)))
            (edges_of_vwalk Pbf)) \<Longrightarrow>
-    not_blocked state (flow_network.oedge e) \<and> 0 < cost_flow_network.rcap (current_flow state) e)"
+    not_blocked state (flow_network_spec.oedge e) \<and> 0 < cost_flow_network.rcap (current_flow state) e)"
     by auto
   have "map (to_edge \<circ>
          (\<lambda>e. prod.fst (local.get_edge_and_costs_forward (not_blocked state) (current_flow state) (prod.fst e)
@@ -2824,7 +2824,7 @@ proof(cases "invar_isOptflow state", goal_cases)
           distinct_map by auto
   have qq_in_E:"set (map cost_flow_network.to_vertex_pair qq) \<subseteq> set es"
     using e_es by auto
-  have qq_in_E':"set (map cost_flow_network.oedge qq) \<subseteq> \<E>" 
+  have qq_in_E':"set (map flow_network_spec.oedge qq) \<subseteq> \<E>" 
     using e_es' by auto
   have not_blocked_qq: "\<And> e . e \<in> set qq \<Longrightarrow> not_blocked state (oedge e)" 
     using  F_is from_aux_invar'(22)[OF knowledge(5)]  qq_prop(4) by fastforce
@@ -2837,9 +2837,9 @@ bf_weight_leq_res_costs:"weight (not_blocked state) (current_flow state) (awalk_
  \<le> foldr (\<lambda>x. (+) (\<cc> x)) qq 0" 
     using qq_in_E not_blocked_qq rcap_qq awalk' qq_len  e_es'
     by(auto intro!: bf_weight_leq_res_costs simp add:  \<E>_def \<E>_impl(1) \<E>_list_def  to_list(1))
-  have oedge_of_EE: "flow_network.oedge ` EEE = \<E>" 
+  have oedge_of_EE: "flow_network_spec.oedge ` EEE = \<E>" 
     by (meson  cost_flow_network.oedge_on_\<EE>)
-  have " cost_flow_network.oedge ` set PP \<subseteq> \<E>"
+  have " flow_network_spec.oedge ` set PP \<subseteq> \<E>"
     using from_aux_invar'(1,3)[OF knowledge(5)] oedge_of_p_allowed by blast
   hence P_in_E: "set PP \<subseteq> EEE"
     by (meson image_subset_iff cost_flow_network.o_edge_res subsetI) 
@@ -2948,7 +2948,7 @@ next
     using "2.prems"(1)  
     by(auto simp add: es_sym[of "(y,x)"] bellman_ford.weight.simps[OF bellman_ford] 2(2) get_edge_and_costs_backward_result_props)
     moreover have "(\<forall>e\<in>set (map (\<lambda>e. prod.fst (get_edge_and_costs_backward nb f (prod.snd e) (prod.fst e))) (map prod.swap (rev ppp))).
-        nb (flow_network.oedge e) \<and> 0 < cost_flow_network.rcap f e)"
+        nb (flow_network_spec.oedge e) \<and> 0 < cost_flow_network.rcap f e)"
       using 2  get_edge_and_costs_backward_result_props[OF prod.collapse[symmetric] _ refl, of nb f x y]
       by auto
     ultimately show ?case by simp
@@ -2975,9 +2975,9 @@ ereal
       by auto
   moreover have "(\<forall>e\<in>set (map (\<lambda>e. prod.fst (get_edge_and_costs_backward nb f (prod.snd e) (prod.fst e)))
                         (map prod.swap (rev (edges_of_vwalk (y # xs))))).
-    nb (flow_network.oedge e) \<and> 0 < cost_flow_network.rcap f e)" 
+    nb (flow_network_spec.oedge e) \<and> 0 < cost_flow_network.rcap f e)" 
     by (simp add: "3.IH" calculation(3))
-  moreover have "nb (flow_network.oedge (prod.fst (get_edge_and_costs_backward nb f x y)))"
+  moreover have "nb (flow_network_spec.oedge (prod.fst (get_edge_and_costs_backward nb f x y)))"
      using 3  get_edge_and_costs_backward_result_props[OF prod.collapse[symmetric] _ refl, of nb f x y]
       by auto
   moreover have "0 < cost_flow_network.rcap f  (prod.fst (get_edge_and_costs_backward nb f x y))"
@@ -3018,7 +3018,7 @@ proof(rule nexistsI, goal_cases)
      0)"
       "(\<And> e. e\<in>set (map (\<lambda>e. prod.fst (get_edge_and_costs_backward (not_blocked state) (current_flow state) (prod.snd e) (prod.fst e)))
              (map prod.swap (rev (edges_of_vwalk c)))) \<Longrightarrow>
-      not_blocked state (flow_network.oedge e) \<and> 0 < cost_flow_network.rcap (current_flow state) e)"
+      not_blocked state (flow_network_spec.oedge e) \<and> 0 < cost_flow_network.rcap (current_flow state) e)"
     using path_bf_flow_network_path_backward[OF _ length_c weight_le_PInfty refl] by auto
   define cc where "cc = (map (\<lambda>e. prod.fst (get_edge_and_costs_backward (not_blocked state) (current_flow state) (prod.snd e) (prod.fst e)))
        (map prod.swap (rev (edges_of_vwalk c))))"
@@ -3112,7 +3112,7 @@ proof(rule if_E[where P= "\<lambda> x. s = x"], fast, goal_cases)
   from 1 have knowledge: "get_target state \<in> VV"
     "aux_invar state"
     "(\<forall>e\<in>to_rdgs to_pair (conv_to_rdg state) (to_graph (\<FF>_imp state)).
-        0 < current_flow state (cost_flow_network.oedge e))"
+        0 < current_flow state (flow_network_spec.oedge e))"
     "invar_isOptflow state" 
     "(\<exists>s\<in>VV. balance state s > (\<epsilon> * current_\<gamma> state) \<and> resreach (current_flow state) s t)"
     using t_prop(1) by auto
@@ -3131,14 +3131,14 @@ proof(rule if_E[where P= "\<lambda> x. s = x"], fast, goal_cases)
   ultimately obtain pp where pp_prop:"augpath (current_flow state) pp"
      "fstv (hd pp) = ss" "sndv (last pp) = t"
      "set pp
-     \<subseteq> {e |e. e \<in> EEE \<and> cost_flow_network.oedge e \<in> to_set (actives state)} \<union> to_rdgs to_pair (conv_to_rdg state) (\<FF> state)"
+     \<subseteq> {e |e. e \<in> EEE \<and> flow_network_spec.oedge e \<in> to_set (actives state)} \<union> to_rdgs to_pair (conv_to_rdg state) (\<FF> state)"
      "foldr (\<lambda>x. (+) (\<cc> x)) pp 0 \<le> foldr (\<lambda>x. (+) (\<cc> x)) p 0"
     using  algo.simulate_inactives_costs[of "current_flow state" p, of ss t state,
                         OF _ _ _ _ _  refl refl refl refl refl refl refl refl]
            1(8) by blast
   have F_is: "\<FF> state = to_graph (\<FF>_imp state)" 
     using knowledge(2) from_aux_invar'(21) by auto
-  hence e_in:"e \<in> set pp \<Longrightarrow> e \<in> {e |e. e \<in> EEE \<and> cost_flow_network.oedge e \<in> to_set (actives state)} 
+  hence e_in:"e \<in> set pp \<Longrightarrow> e \<in> {e |e. e \<in> EEE \<and> flow_network_spec.oedge e \<in> to_set (actives state)} 
                    \<union> to_rdgs to_pair (conv_to_rdg state) (\<FF> state)" for e
       using pp_prop(4)  by auto
     hence e_es:"e \<in> set pp \<Longrightarrow> cost_flow_network.to_vertex_pair e \<in> set es" for e
@@ -3155,7 +3155,7 @@ proof(rule if_E[where P= "\<lambda> x. s = x"], fast, goal_cases)
       using oedge_where from_aux_invar'(1,3)[OF knowledge(2)] by auto
     have posflow:"\<exists> d. e = B d \<Longrightarrow> current_flow state (oedge e) > 0" 
       using cost_flow_network.augpath_rcap_pos_strict'[OF  pp_prop(1) 1]
-      by(induction  rule: cost_flow_network.oedge.cases[OF  , of e])
+      by(induction  rule: flow_network_spec.oedge.cases[OF  , of e])
          auto
     have "prod.snd (get_edge_and_costs_backward (not_blocked state) (current_flow state)
      (sndv e) (fstv e)) \<le> \<cc> e"
@@ -3242,7 +3242,7 @@ proof(rule if_E[where P= "\<lambda> x. s = x"], fast, goal_cases)
      0) \<and>
   (\<forall>e\<in>set (map (\<lambda>e. prod.fst (get_edge_and_costs_backward (not_blocked state) (current_flow state) (prod.snd e) (prod.fst e)))
              (map prod.swap (rev (edges_of_vwalk Pbf)))).
-      not_blocked state (cost_flow_network.oedge e) \<and> 0 < cost_flow_network.rcap (current_flow state) e)"
+      not_blocked state (flow_network_spec.oedge e) \<and> 0 < cost_flow_network.rcap (current_flow state) e)"
    using path_bf_flow_network_path_backward[OF _ length_Pbf weight_le_PInfty refl] by simp
    hence Pbf_props: "awalk UNIV (last Pbf) (map prod.swap (rev (edges_of_vwalk Pbf))) (hd Pbf)"
                    "weight_backward (not_blocked state) (current_flow state) Pbf =
@@ -3253,7 +3253,7 @@ proof(rule if_E[where P= "\<lambda> x. s = x"], fast, goal_cases)
      0)"
          "(\<And> e. e  \<in>set (map (\<lambda>e. prod.fst (get_edge_and_costs_backward (not_blocked state) (current_flow state) (prod.snd e) (prod.fst e)))
              (map prod.swap (rev (edges_of_vwalk Pbf)))) \<Longrightarrow>
-      not_blocked state (cost_flow_network.oedge e) \<and> 0 < cost_flow_network.rcap (current_flow state) e)"
+      not_blocked state (flow_network_spec.oedge e) \<and> 0 < cost_flow_network.rcap (current_flow state) e)"
     by auto
   define P where "P = (map (\<lambda>e. prod.fst (get_edge_and_costs_backward (not_blocked state) (current_flow state) (prod.snd e) (prod.fst e)))
              (map prod.swap (rev (edges_of_vwalk Pbf))))"
@@ -3347,8 +3347,8 @@ next
 qed
 
 lemma bf_weight_backward_leq_res_costs:
-assumes "set (map cost_flow_network.oedge qq) \<subseteq> \<E>"
-    " \<And> e. e \<in> set qq \<Longrightarrow> not_blocked state (cost_flow_network.oedge e)"
+assumes "set (map flow_network_spec.oedge qq) \<subseteq> \<E>"
+    " \<And> e. e \<in> set qq \<Longrightarrow> not_blocked state (flow_network_spec.oedge e)"
     "\<And> e. e \<in> set qq \<Longrightarrow> 0 < cost_flow_network.rcap (current_flow state) e"
     "unconstrained_awalk (map cost_flow_network.to_vertex_pair qq)"
    and  qq_len: "length qq \<ge> 1"
@@ -3479,7 +3479,7 @@ lemma get_source_target_path_b_ax:
   assumes "get_source_target_path_b_cond  state s t P b \<gamma> f"
   shows "0 < cost_flow_network.Rcap f (set P) \<and>
         (invar_isOptflow state \<longrightarrow> cost_flow_network.is_min_path f s t P) \<and>
-         cost_flow_network.oedge ` set P \<subseteq> to_set (actives state) \<union> \<F> state \<and>
+         flow_network_spec.oedge ` set P \<subseteq> to_set (actives state) \<union> \<F> state \<and>
          distinct P"
   apply(insert assms)
   unfolding  loopB.get_source_target_path_b_cond_def
@@ -3514,7 +3514,7 @@ proof(cases "invar_isOptflow state", goal_cases)
        (insert"1"(1) , unfold get_source_for_target_def, presburger+)  
   hence 
     "(\<forall>e\<in>to_rdgs to_pair (conv_to_rdg state) (to_graph  (\<FF>_imp state)).
-        0 < current_flow state (cost_flow_network.oedge e))"
+        0 < current_flow state (flow_network_spec.oedge e))"
     by auto
   have s_prop: "b s > \<epsilon> * \<gamma>" "resreach f s t" 
     using get_source_for_target_ax[OF knowledge (8,9,12,10,11) loopB_call2_cond knowledge(13)]
@@ -3541,7 +3541,7 @@ proof(cases "invar_isOptflow state", goal_cases)
      "fstv (hd qq) = s"
      "sndv (last qq) = t"
      "set qq
-     \<subseteq> {e |e. e \<in> EEE \<and> cost_flow_network.oedge e \<in> to_set (actives state)} \<union>
+     \<subseteq> {e |e. e \<in> EEE \<and> flow_network_spec.oedge e \<in> to_set (actives state)} \<union>
         to_rdgs to_pair (conv_to_rdg state) (\<FF> state)"
      "foldr (\<lambda>x. (+) (\<cc> x)) qq 0 \<le> foldr (\<lambda>x. (+) (\<cc> x)) Q 0" "qq \<noteq> []"
   using algo.simulate_inactives_costs[OF Q_prop(1-4) knowledge(5)
@@ -3554,10 +3554,10 @@ proof(cases "invar_isOptflow state", goal_cases)
     by (simp add: "1"(1) from_aux_invar'(21))
   have consist: "cost_flow_network.consist (conv_to_rdg state)" 
     using from_aux_invar'(6) knowledge(5) by auto
-  hence "e \<in> set qq \<Longrightarrow> e \<in> {e |e. e \<in> EEE \<and> cost_flow_network.oedge e \<in> to_set (actives state)} 
+  hence "e \<in> set qq \<Longrightarrow> e \<in> {e |e. e \<in> EEE \<and> flow_network_spec.oedge e \<in> to_set (actives state)} 
                    \<union> to_rdgs to_pair (conv_to_rdg state) (\<FF> state)" for e
     using qq_prop(4)  by auto
- hence e_in:"e \<in> set (map cost_flow_network.erev (rev qq)) \<Longrightarrow> e \<in> {e |e. e \<in> EEE \<and> cost_flow_network.oedge e \<in> to_set (actives state)} 
+ hence e_in:"e \<in> set (map cost_flow_network.erev (rev qq)) \<Longrightarrow> e \<in> {e |e. e \<in> EEE \<and> flow_network_spec.oedge e \<in> to_set (actives state)} 
                    \<union> to_rdgs to_pair (conv_to_rdg state) (\<FF> state)" for e
    using cost_flow_network.Residuals_project_erev_sym Forest_conv_erev_sym[OF consist] by (auto, blast, meson)
     hence e_es:"e \<in> set (map cost_flow_network.erev (rev qq)) \<Longrightarrow> oedge e \<in> \<E>" for e
@@ -3580,7 +3580,7 @@ proof(cases "invar_isOptflow state", goal_cases)
       using oedgeF  from_aux_invar'(22)[OF knowledge(5)] by auto
     moreover have flowpos:"\<exists> d. (cost_flow_network.erev e) = B d\<Longrightarrow> current_flow state (oedge (cost_flow_network.erev e)) > 0" 
       using cost_flow_network.augpath_rcap_pos_strict'[OF  qq_prop(1) 11] knowledge(12)
-      by(induction rule: cost_flow_network.oedge.cases[OF  , of e])
+      by(induction rule: flow_network_spec.oedge.cases[OF  , of e])
       auto  
       ultimately show ?case 
         using "11" cost_flow_network.augpath_rcap_pos_strict cost_flow_network.oedge_and_reversed cost_flow_network.vs_erev
@@ -3664,7 +3664,7 @@ proof(cases "invar_isOptflow state", goal_cases)
          (\<forall>e\<in>set (map (\<lambda>e. prod.fst (get_edge_and_costs_backward(not_blocked state) (current_flow state) (prod.snd e)
                          (prod.fst e)))
            (map prod.swap (rev (edges_of_vwalk (rev Pbf)))) ).
-    not_blocked state (cost_flow_network.oedge e) \<and> 0 < cost_flow_network.rcap (current_flow state) e)"
+    not_blocked state (flow_network_spec.oedge e) \<and> 0 < cost_flow_network.rcap (current_flow state) e)"
     using path_bf_flow_network_path_backward[OF _ length_Pbf[simplified sym[OF length_rev[of Pbf]]]
                     weight_le_PInfty refl, simplified last_rev hd_rev] by simp
     hence Pbf_props: "awalk UNIV (hd Pbf) (edges_of_vwalk  Pbf)  (last Pbf)"
@@ -3675,7 +3675,7 @@ proof(cases "invar_isOptflow state", goal_cases)
          "\<And> e. e\<in>set (map (\<lambda>e. prod.fst (get_edge_and_costs_backward(not_blocked state) (current_flow state) (prod.snd e)
                          (prod.fst e)))
            ( edges_of_vwalk  Pbf) ) \<Longrightarrow>
-    not_blocked state (cost_flow_network.oedge e) \<and> 0 < cost_flow_network.rcap (current_flow state) e"
+    not_blocked state (flow_network_spec.oedge e) \<and> 0 < cost_flow_network.rcap (current_flow state) e"
       using edges_of_vwalk_rev_swap[of "rev Pbf"] 
       by auto 
   have same_edges:"(map cost_flow_network.to_vertex_pair PP) = (edges_of_vwalk Pbf)"
@@ -3726,9 +3726,9 @@ proof(cases "invar_isOptflow state", goal_cases)
   have distinctP:"distinct PP" 
     using distinct_edges_of_vwalk[OF distinct_Pbf, simplified sym[OF same_edges ]]
           distinct_map by auto
-  have qq_in_E:"set (map cost_flow_network.oedge (map cost_flow_network.erev (rev qq))) \<subseteq> \<E>"
+  have qq_in_E:"set (map flow_network_spec.oedge (map cost_flow_network.erev (rev qq))) \<subseteq> \<E>"
     using e_es by auto
-  hence qq_rev_in_E:"set ( map cost_flow_network.oedge qq) \<subseteq> \<E>" 
+  hence qq_rev_in_E:"set ( map flow_network_spec.oedge qq) \<subseteq> \<E>" 
     by(auto simp add: es_sym image_subset_iff cost_flow_network.oedge_and_reversed)
   have not_blocked_qq: "\<And> e . e \<in> set qq \<Longrightarrow> not_blocked state (oedge e)" 
     using  F_is from_aux_invar'(22)[OF knowledge(5)]  qq_prop(4) by fastforce
@@ -3744,9 +3744,9 @@ bf_weight_leq_res_costs:"weight_backward (not_blocked state) (current_flow state
  \<le> foldr (\<lambda>x. (+) (\<cc> x)) qq 0" 
     using qq_rev_in_E not_blocked_qq rcap_qq awalk'  qq_len 
     by(fastforce intro!: bf_weight_backward_leq_res_costs[simplified cost_flow_network.rev_erev_swap , simplified rev_map, of qq state t])   
-  have oedge_of_EE: "flow_network.oedge ` EEE = \<E>" 
+  have oedge_of_EE: "flow_network_spec.oedge ` EEE = \<E>" 
     by (meson cost_flow_network.oedge_on_\<EE>)
-  have " cost_flow_network.oedge ` set PP \<subseteq> \<E>"
+  have " flow_network_spec.oedge ` set PP \<subseteq> \<E>"
     using from_aux_invar'(1,3)[OF knowledge(5)] oedge_of_p_allowed by blast
   hence P_in_E: "set PP \<subseteq> EEE"
     by (meson image_subset_iff cost_flow_network.o_edge_res subsetI) 
@@ -4232,7 +4232,7 @@ proof(goal_cases)
                   (prod.fst e) (prod.snd e)))
              (edges_of_vwalk (p @ [x])))"
     have transformed:" awalk UNIV (hd (p @ [x])) (edges_of_vwalk (p @ [x])) (last (p @ [x]))"
-         "(\<And>e. e\<in>set pp \<Longrightarrow> not_blocked state (cost_flow_network.oedge e) \<and> 0 < cost_flow_network.rcap (current_flow state) e)"
+         "(\<And>e. e\<in>set pp \<Longrightarrow> not_blocked state (flow_network_spec.oedge e) \<and> 0 < cost_flow_network.rcap (current_flow state) e)"
       using path_bf_flow_network_path[OF _ _ pw_le_PInfty refl] p_prop pp_def by auto
     have path_hd: "hd (p @ [x]) = fstv (hd pp)"
       by(subst  pp_def , subst hd_map, ((insert p_prop(4), cases p rule: list_cases3, auto)[1]),
@@ -4278,14 +4278,14 @@ proof(goal_cases)
     then obtain qq where qq_props:"augpath f qq"
        "fstv (hd qq) = s"
        "sndv (last qq) = t"
-       "set qq \<subseteq> {e |e. e \<in> EEE \<and> cost_flow_network.oedge e \<in> to_set (actives state)}
+       "set qq \<subseteq> {e |e. e \<in> EEE \<and> flow_network_spec.oedge e \<in> to_set (actives state)}
             \<union> to_rdgs to_pair (conv_to_rdg state) (\<FF> state)"
        "qq \<noteq> []"
     using algo.simulate_inactives[OF q_props(1-4) 1(5) refl 1(3) refl refl refl refl refl refl _  1(6)]
         t_not_s by auto
-    have e_in_qq_not_blocked: "e \<in> set qq \<Longrightarrow> not_blocked state (cost_flow_network.oedge e)" for e   
+    have e_in_qq_not_blocked: "e \<in> set qq \<Longrightarrow> not_blocked state (flow_network_spec.oedge e)" for e   
       using qq_props(4) 
-      by(induction e rule: cost_flow_network.oedge.induct)
+      by(induction e rule: flow_network_spec.oedge.induct)
         (force simp add: spec[OF from_aux_invar'(22)[OF 1(5)]] from_aux_invar'(21)[OF 1(5)])+
     have e_in_qq_rcap: "e \<in> set qq \<Longrightarrow> 0 < cost_flow_network.rcap f e" for e
       using qq_props(1)  linorder_class.Min_gr_iff 
@@ -4454,7 +4454,7 @@ proof(goal_cases)
     define pp where "pp = (map (\<lambda>e. prod.fst (get_edge_and_costs_backward (not_blocked state) (current_flow state) (prod.snd e) (prod.fst e)))
                (map prod.swap (rev (edges_of_vwalk (p @ [x])))))"
     have transformed:" awalk UNIV (last (p @ [x])) (map prod.swap (rev (edges_of_vwalk (p @ [x])))) (hd (p @ [x]))"
-         "(\<And>e. e\<in>set pp \<Longrightarrow> not_blocked state (cost_flow_network.oedge e) \<and> 0 < cost_flow_network.rcap (current_flow state) e)"
+         "(\<And>e. e\<in>set pp \<Longrightarrow> not_blocked state (flow_network_spec.oedge e) \<and> 0 < cost_flow_network.rcap (current_flow state) e)"
       using path_bf_flow_network_path_backward[OF _ _ pw_le_PInfty refl] p_prop pp_def by auto
     have non_empt: "(rev (edges_of_vwalk (p @ [x]))) \<noteq> []"
       by(insert p_prop(4); cases p rule: list_cases3; auto)
@@ -4497,14 +4497,14 @@ proof(goal_cases)
     then obtain qq where qq_props:"augpath f qq"
        "fstv (hd qq) = s"
        "sndv (last qq) = t"
-       "set qq \<subseteq> {e |e. e \<in> EEE \<and> cost_flow_network.oedge e \<in> to_set (actives state)}
+       "set qq \<subseteq> {e |e. e \<in> EEE \<and> flow_network_spec.oedge e \<in> to_set (actives state)}
             \<union> to_rdgs to_pair (conv_to_rdg state) (\<FF> state)"
        "qq \<noteq> []"
     using algo.simulate_inactives[OF  q_props(1-4) 1(5) refl 1(3) refl refl refl refl refl refl _  1(6)]
         t_not_s by auto
-    have e_in_qq_not_blocked: "e \<in> set qq \<Longrightarrow> not_blocked state (flow_network.oedge e)" for e   
+    have e_in_qq_not_blocked: "e \<in> set qq \<Longrightarrow> not_blocked state (flow_network_spec.oedge e)" for e   
       using qq_props(4) 
-      by(induction e rule: cost_flow_network.oedge.induct)
+      by(induction e rule: flow_network_spec.oedge.induct)
         (force simp add: spec[OF from_aux_invar'(22)[OF 1(5)]] from_aux_invar'(21)[OF 1(5)])+
     have e_in_qq_rcap: "e \<in> set qq \<Longrightarrow> 0 < cost_flow_network.rcap f e" for e
       using qq_props(1)  linorder_class.Min_gr_iff 
